translator now works for pure subset in ref semantics

translator/ml_optimiseScript.sml
@@ -45,6 +45,7 @@ val BOTTOM_UP_OPT_def = tDefine "BOTTOM_UP_OPT" `
   (BOTTOM_UP_OPT f (Var name) = f (Var name)) /\
   (BOTTOM_UP_OPT f (Con tag xs) = f (Con tag (MAP (BOTTOM_UP_OPT f) xs))) /\
   (BOTTOM_UP_OPT f (Fun name x) = f (Fun name x)) /\
+  (BOTTOM_UP_OPT f (Uapp uop x2) = f (Uapp uop (BOTTOM_UP_OPT f x2))) /\
   (BOTTOM_UP_OPT f (App op x1 x2) = f (App op (BOTTOM_UP_OPT f x1) (BOTTOM_UP_OPT f x2))) /\
   (BOTTOM_UP_OPT f (Log l x1 x2) = f (Log l (BOTTOM_UP_OPT f x1) (BOTTOM_UP_OPT f x2))) /\
   (BOTTOM_UP_OPT f (If x1 x2 x3) = f (If (BOTTOM_UP_OPT f x1) (BOTTOM_UP_OPT f x2) (BOTTOM_UP_OPT f x3))) /\
@@ -59,10 +60,10 @@ val two_assums = METIS_PROVE [] ``(b ==> c) = (b ==> c /\ b)``;
 val isRval_def = Define `(isRval (Rval _) = T) /\ (isRval _ = F)`;
 
 val BOTTOM_UP_OPT_LEMMA = prove(
-  ``(!env exp res. evaluate' env exp res ==> isRval res ==> evaluate' env (f exp) res) ==>
-    (!x1 x2 x3. evaluate' x1 x2 x3 ==> isRval x3 ==> evaluate' x1 (BOTTOM_UP_OPT f x2) x3) /\
-    (!x1 x2 x3. evaluate_list' x1 x2 x3 ==> isRval x3 ==> evaluate_list' x1 (MAP (BOTTOM_UP_OPT f) x2) x3) /\
-    (!x1 x2 x3 x4. evaluate_match' x1 x2 x3 x4 ==> isRval x4 ==> evaluate_match' x1 x2 (MAP (\(p,x). (p,BOTTOM_UP_OPT f x)) x3) x4)``,
+  ``(!s env exp res. evaluate' s env exp res ==> isRval res ==> evaluate' s env (f exp) res) ==>
+    (!s x1 x2 x3. evaluate' s x1 x2 x3 ==> isRval x3 ==> evaluate' s x1 (BOTTOM_UP_OPT f x2) x3) /\
+    (!s x1 x2 x3. evaluate_list' s x1 x2 x3 ==> isRval x3 ==> evaluate_list' s x1 (MAP (BOTTOM_UP_OPT f) x2) x3) /\
+    (!s x1 x2 x3 x4. evaluate_match' s x1 x2 x3 x4 ==> isRval x4 ==> evaluate_match' s x1 x2 (MAP (\(p,x). (p,BOTTOM_UP_OPT f x)) x3) x4)``,
   STRIP_TAC \\ ONCE_REWRITE_TAC [two_assums]
   \\ HO_MATCH_MP_TAC evaluate'_ind \\ REPEAT STRIP_TAC
   \\ FULL_SIMP_TAC std_ss [BOTTOM_UP_OPT_def,isRval_def,AND_IMP_INTRO]
@@ -71,16 +72,24 @@ val BOTTOM_UP_OPT_LEMMA = prove(
   \\ TRY (Q.PAT_ASSUM `!x.bbb` (fn th => MATCH_MP_TAC th THEN ASSUME_TAC th)
           THEN ASM_SIMP_TAC (srw_ss()) [Once evaluate'_cases,isRval_def] THEN NO_TAC)
   THEN1 (Q.PAT_ASSUM `!x.bbb` (fn th => MATCH_MP_TAC th \\ ASSUME_TAC th)
+    \\ ASM_SIMP_TAC (srw_ss()) [Once evaluate'_cases,isRval_def]
+    \\ REPEAT DISJ1_TAC \\ Q.LIST_EXISTS_TAC [`v`]
+    \\ ASM_SIMP_TAC std_ss [] \\ METIS_TAC [])
+  THEN1
+   (ASM_SIMP_TAC (srw_ss()) [Once evaluate'_cases,isRval_def]
+    \\ REPEAT DISJ1_TAC
+    \\ Q.LIST_EXISTS_TAC [`v`,`s2`] \\ ASM_SIMP_TAC std_ss [])
+  THEN1
+   (ASM_SIMP_TAC (srw_ss()) [Once evaluate'_cases,isRval_def]
+    \\ REPEAT DISJ1_TAC
+    \\ Q.LIST_EXISTS_TAC [`v`,`s2`] \\ ASM_SIMP_TAC std_ss [])
+  THEN1 (Q.PAT_ASSUM `!x.bbb` (fn th => MATCH_MP_TAC th \\ ASSUME_TAC th)
     \\ ASM_SIMP_TAC (srw_ss()) [Once evaluate'_cases]
     \\ REPEAT DISJ1_TAC \\ Q.LIST_EXISTS_TAC [`v1`,`v2`]
-    \\ ASM_SIMP_TAC std_ss [])
-  THEN1 (ASM_SIMP_TAC (srw_ss()) [Once evaluate'_cases]
-    \\ REPEAT DISJ1_TAC \\ Q.LIST_EXISTS_TAC [`v1`,`v2`]
-    \\ ASM_SIMP_TAC std_ss [])
-  THEN1 (ASM_SIMP_TAC (srw_ss()) [Once evaluate'_cases]
-    \\ DISJ2_TAC \\ REPEAT DISJ1_TAC \\ Q.LIST_EXISTS_TAC [`v1`,`v2`]
-    \\ ASM_SIMP_TAC std_ss [])
-  THEN1 (ASM_SIMP_TAC (srw_ss()) [Once evaluate'_cases] \\ METIS_TAC [])
+    \\ ASM_SIMP_TAC std_ss [] \\ METIS_TAC [])
+  THEN1 (ASM_SIMP_TAC (srw_ss()) [Once evaluate'_cases,isRval_def] \\ METIS_TAC [])
+  THEN1 (ASM_SIMP_TAC (srw_ss()) [Once evaluate'_cases,isRval_def] \\ METIS_TAC [])
+  THEN1 (ASM_SIMP_TAC (srw_ss()) [Once evaluate'_cases,isRval_def] \\ METIS_TAC [])
   THEN1 (Q.PAT_ASSUM `!x.bbb` (fn th => MATCH_MP_TAC th \\ ASSUME_TAC th)
     \\ ASM_SIMP_TAC (srw_ss()) [Once evaluate'_cases]
     \\ DISJ1_TAC \\ Q.EXISTS_TAC `v` \\ FULL_SIMP_TAC std_ss []
@@ -88,45 +97,37 @@ val BOTTOM_UP_OPT_LEMMA = prove(
     \\ Cases_on `op` \\ FULL_SIMP_TAC (srw_ss()) []
     \\ Cases_on `v` \\ FULL_SIMP_TAC (srw_ss()) []
     \\ Cases_on `l` \\ FULL_SIMP_TAC (srw_ss()) []
-    \\ Cases_on `b` \\ FULL_SIMP_TAC (srw_ss()) [])
-  THEN1 (ASM_SIMP_TAC (srw_ss()) [Once evaluate'_cases]
-    \\ DISJ1_TAC \\ Q.EXISTS_TAC `v`
-    \\ FULL_SIMP_TAC std_ss [do_log_def])
-  THEN1 (ASM_SIMP_TAC (srw_ss()) [Once evaluate'_cases]
-    \\ DISJ2_TAC \\ DISJ1_TAC \\ Q.EXISTS_TAC `v`
-    \\ FULL_SIMP_TAC std_ss [do_log_def])
+    \\ Cases_on `b` \\ FULL_SIMP_TAC (srw_ss()) [] \\ METIS_TAC [])
+  THEN1 (ASM_SIMP_TAC (srw_ss()) [Once evaluate'_cases,isRval_def] \\ METIS_TAC [])
+  THEN1 (ASM_SIMP_TAC (srw_ss()) [Once evaluate'_cases,isRval_def] \\ METIS_TAC [])
   THEN1 (Q.PAT_ASSUM `!x.bbb` (fn th => MATCH_MP_TAC th \\ ASSUME_TAC th)
     \\ ASM_SIMP_TAC (srw_ss()) [Once evaluate'_cases]
     \\ DISJ1_TAC \\ Q.EXISTS_TAC `v`
     \\ FULL_SIMP_TAC std_ss [do_if_def]
     \\ REPEAT (BasicProvers.FULL_CASE_TAC)
     \\ FULL_SIMP_TAC (srw_ss()) [] \\ METIS_TAC [])
-  THEN1 (ASM_SIMP_TAC (srw_ss()) [Once evaluate'_cases]
-    \\ DISJ1_TAC \\ Q.EXISTS_TAC `v`
-    \\ FULL_SIMP_TAC std_ss [do_if_def]
-    \\ REPEAT (BasicProvers.FULL_CASE_TAC)
-    \\ FULL_SIMP_TAC (srw_ss()) [] \\ METIS_TAC [])
-  THEN1 (ASM_SIMP_TAC (srw_ss()) [Once evaluate'_cases]
-    \\ DISJ2_TAC \\ DISJ1_TAC \\ Q.EXISTS_TAC `v`
-    \\ FULL_SIMP_TAC std_ss [do_if_def]
-    \\ REPEAT (BasicProvers.FULL_CASE_TAC)
-    \\ FULL_SIMP_TAC (srw_ss()) [] \\ METIS_TAC [])
+  THEN1 (ASM_SIMP_TAC (srw_ss()) [Once evaluate'_cases,isRval_def] \\ METIS_TAC [])
+  THEN1 (ASM_SIMP_TAC (srw_ss()) [Once evaluate'_cases,isRval_def] \\ METIS_TAC [])
   THEN1 (Q.PAT_ASSUM `!x.bbb` (fn th => MATCH_MP_TAC th \\ ASSUME_TAC th)
     \\ ASM_SIMP_TAC (srw_ss()) [Once evaluate'_cases] \\ METIS_TAC [])
-  THEN1 (ASM_SIMP_TAC (srw_ss()) [Once evaluate'_cases] \\ METIS_TAC [])
+  THEN1 (ASM_SIMP_TAC (srw_ss()) [Once evaluate'_cases,isRval_def] \\ METIS_TAC [])
   THEN1 (Q.PAT_ASSUM `!x.bbb` (fn th => MATCH_MP_TAC th \\ ASSUME_TAC th)
     \\ ASM_SIMP_TAC (srw_ss()) [Once evaluate'_cases] \\ METIS_TAC [])
-  THEN1 (ASM_SIMP_TAC (srw_ss()) [Once evaluate'_cases] \\ METIS_TAC [])
-  THEN1 (ASM_SIMP_TAC (srw_ss()) [Once evaluate'_cases] \\ METIS_TAC []));
+  THEN1 (ASM_SIMP_TAC (srw_ss()) [Once evaluate'_cases,isRval_def] \\ METIS_TAC [])
+  THEN1 (ASM_SIMP_TAC (srw_ss()) [Once evaluate'_cases,isRval_def] \\ METIS_TAC [])
+  THEN1 (ASM_SIMP_TAC (srw_ss()) [Once evaluate'_cases,isRval_def] \\ METIS_TAC [])
+  THEN1 (ASM_SIMP_TAC (srw_ss()) [Once evaluate'_cases,isRval_def] \\ METIS_TAC []));
 
 val BOTTOM_UP_OPT_THM = prove(
   ``!f.
-      (!env exp res.
-         evaluate' env exp (Rval res) ==> evaluate' env (f exp) (Rval res)) ==>
-      (!env exp res.
-         evaluate' env exp (Rval res) ==> evaluate' env (BOTTOM_UP_OPT f exp) (Rval res))``,
+      (!s env exp res.
+         evaluate' s env exp (Rval res) ==>
+         evaluate' s env (f exp) (Rval res)) ==>
+      (!s env exp res.
+         evaluate' s env exp (Rval res) ==>
+         evaluate' s env (BOTTOM_UP_OPT f exp) (Rval res))``,
   STRIP_TAC \\ STRIP_TAC \\ (BOTTOM_UP_OPT_LEMMA
-    |> UNDISCH |> CONJUNCT1 |> Q.SPECL [`env`,`exp`,`Rval res`] |> GEN_ALL
+    |> UNDISCH |> CONJUNCT1 |> Q.SPECL [`s`,`env`,`exp`,`Rval res`] |> GEN_ALL
     |> DISCH_ALL |> GEN_ALL |> SIMP_RULE std_ss [isRval_def] |> MATCH_MP_TAC)
   \\ REPEAT STRIP_TAC \\ Cases_on `res` \\ FULL_SIMP_TAC std_ss [isRval_def])
   |> SIMP_RULE std_ss [PULL_FORALL,AND_IMP_INTRO];
@@ -140,15 +141,15 @@ val abs2let_def = Define `
              | rest => rest`;
 
 val abs2let_thm = prove(
-  ``!env exp res. evaluate' env exp (Rval res) ==>
-                  evaluate' env (abs2let exp) (Rval res)``,
+  ``!s env exp res. evaluate' s env exp (Rval res) ==>
+                    evaluate' s env (abs2let exp) (Rval res)``,
   SIMP_TAC std_ss [abs2let_def] \\ REPEAT STRIP_TAC
   \\ REPEAT (BasicProvers.FULL_CASE_TAC)
   \\ ASM_SIMP_TAC std_ss [] \\ POP_ASSUM MP_TAC
   \\ SIMP_TAC (srw_ss()) [Once evaluate'_cases,do_app_def]
   \\ REPEAT STRIP_TAC \\ SIMP_TAC (srw_ss()) [Once evaluate'_cases]
-  \\ Q.EXISTS_TAC `v2` \\ FULL_SIMP_TAC std_ss []
-  \\ Q.PAT_ASSUM `evaluate' env (Fun s e') (Rval v1)` MP_TAC
+  \\ Q.LIST_EXISTS_TAC [`v2`,`s3`] \\ FULL_SIMP_TAC std_ss []
+  \\ Q.PAT_ASSUM `evaluate' s env (Fun s' e') (Rval (s2,v1))` MP_TAC
   \\ SIMP_TAC (srw_ss()) [Once evaluate'_cases,do_app_def]
   \\ REPEAT STRIP_TAC \\ FULL_SIMP_TAC (srw_ss()) []);
 
@@ -160,9 +161,9 @@ val let_id_def = Define `
   (let_id rest = rest)`;
 
 val let_id_thm = prove(
-  ``!env exp res. evaluate' env exp (Rval res) ==>
-                  evaluate' env (let_id exp) (Rval res)``,
-  STRIP_TAC \\ HO_MATCH_MP_TAC (fetch "-" "let_id_ind")
+  ``!s env exp res. evaluate' s env exp (Rval res) ==>
+                    evaluate' s env (let_id exp) (Rval res)``,
+  STRIP_TAC \\ STRIP_TAC \\ HO_MATCH_MP_TAC (fetch "-" "let_id_ind")
   \\ FULL_SIMP_TAC std_ss [let_id_def] \\ SRW_TAC [] [] \\ POP_ASSUM MP_TAC
   \\ SIMP_TAC (srw_ss()) [Once evaluate'_cases]
   \\ REPEAT STRIP_TAC \\ POP_ASSUM MP_TAC
@@ -182,12 +183,12 @@ val opt_sub_add_def = Define `
      | NONE => x
      | (SOME (op1,y,z)) =>
         case dest_binop y of
-         | NONE => x
-         | (SOME (op2,x1,y1)) =>
-            if z = y1 then
+         | (SOME (op2,x1,Lit y1)) =>
+            if z = Lit y1 then
               if (op1 = Plus) /\ (op2 = Minus) then x1 else
               if (op2 = Plus) /\ (op1 = Minus) then x1 else x
-            else x`;
+            else x
+         | _ => x`;
 
 val dest_binop_thm = prove(
   ``!x. (dest_binop x = SOME (x1,x2,x3)) ==> (x = App (Opn x1) x2 x3)``,
@@ -195,45 +196,50 @@ val dest_binop_thm = prove(
   \\ FULL_SIMP_TAC (srw_ss()) [dest_binop_def]);
 
 val do_app_IMP = prove(
-  ``(do_app env (Opn opn) v1 v2 = SOME (env1,e3)) ==>
+  ``(do_app s env (Opn opn) v1 v2 = SOME (s1,env1,e3)) ==>
     ?i1 i2. (v1 = Litv (IntLit i1)) /\ (v2 = Litv (IntLit i2))``,
   FULL_SIMP_TAC (srw_ss()) [do_app_def]
   \\ REPEAT (BasicProvers.FULL_CASE_TAC)
   \\ FULL_SIMP_TAC (srw_ss()) []);
 
 val evaluate'_11_Rval = prove(
-  ``evaluate' env exp (Rval res1) ==>
-    evaluate' env exp (Rval res2) ==> (res1 = res2)``,
+  ``evaluate' s env exp (Rval res1) ==>
+    evaluate' s env exp (Rval res2) ==> (res1 = res2)``,
   REPEAT STRIP_TAC \\ IMP_RES_TAC big_exp_determ'
   \\ FULL_SIMP_TAC (srw_ss()) []);
 
 val evaluate_Lit = prove(
-  ``evaluate' env (Lit l) (Rval res) = (res = Litv l)``,
-  FULL_SIMP_TAC (srw_ss()) [Once evaluate'_cases]);
+  ``evaluate' s env (Lit l) (Rval (s1,res)) = (res = Litv l) /\ (s = s1)``,
+  FULL_SIMP_TAC (srw_ss()) [Once evaluate'_cases] \\ METIS_TAC []);
 
 val opt_sub_add_thm = prove(
-  ``!env exp res. evaluate' env exp (Rval res) ==>
-                  evaluate' env (opt_sub_add exp) (Rval res)``,
-  STRIP_TAC \\ STRIP_TAC \\ SIMP_TAC std_ss [opt_sub_add_def]
+  ``!s env exp res. evaluate' s env exp (Rval res) ==>
+                    evaluate' s env (opt_sub_add exp) (Rval res)``,
+  STRIP_TAC \\ STRIP_TAC \\ STRIP_TAC \\ SIMP_TAC std_ss [opt_sub_add_def]
   \\ Cases_on `dest_binop exp` \\ FULL_SIMP_TAC std_ss []
   \\ `?x1 x2 x3. x = (x1,x2,x3)` by METIS_TAC [PAIR]
   \\ FULL_SIMP_TAC (srw_ss()) []
   \\ Cases_on `dest_binop x2` \\ FULL_SIMP_TAC std_ss []
   \\ `?y1 y2 y3. x' = (y1,y2,y3)` by METIS_TAC [PAIR]
   \\ FULL_SIMP_TAC (srw_ss()) [] \\ SRW_TAC [] []
+  \\ Cases_on `y3` \\ FULL_SIMP_TAC (srw_ss()) []
+  \\ Cases_on `x3 = Lit l` \\ FULL_SIMP_TAC std_ss []
   \\ IMP_RES_TAC dest_binop_thm \\ FULL_SIMP_TAC std_ss []
-  \\ POP_ASSUM (K ALL_TAC) \\ POP_ASSUM (K ALL_TAC) \\ POP_ASSUM MP_TAC
+  \\ POP_ASSUM (K ALL_TAC) \\ POP_ASSUM (K ALL_TAC)
+  \\ POP_ASSUM (K ALL_TAC) \\ POP_ASSUM MP_TAC
   \\ SIMP_TAC (srw_ss()) [Once evaluate'_cases]
   \\ SIMP_TAC (srw_ss()) [Once evaluate'_cases]
   \\ REPEAT STRIP_TAC
+  \\ FULL_SIMP_TAC (srw_ss()) [evaluate_Lit]
   \\ `?i1 i2. (v1 = Litv (IntLit i1)) /\ (v2 = Litv (IntLit i2))` by METIS_TAC [do_app_IMP]
   \\ `?i1' i2'. (v1' = Litv (IntLit i1')) /\ (v2' = Litv (IntLit i2'))` by METIS_TAC [do_app_IMP]
   \\ FULL_SIMP_TAC std_ss []
   \\ FULL_SIMP_TAC (srw_ss()) [do_app_def]
   \\ REPEAT (Q.PAT_ASSUM `Lit xx = yy` (ASSUME_TAC o GSYM))
+  \\ Cases_on `res`
   \\ FULL_SIMP_TAC (srw_ss()) [evaluate_Lit]
-  \\ Q.PAT_ASSUM `env' = env''` (fn th => FULL_SIMP_TAC std_ss [th])
-  \\ IMP_RES_TAC evaluate'_11_Rval \\ FULL_SIMP_TAC (srw_ss()) []
+  \\ REPEAT (Q.PAT_ASSUM `IntLit xx = yy` (ASSUME_TAC o GSYM))
+  \\ FULL_SIMP_TAC (srw_ss()) [evaluate_Lit]
   \\ FULL_SIMP_TAC (srw_ss()) [opn_lookup_def,
        intLib.COOPER_PROVE ``i + i2 − i2 = i:int``,
        intLib.COOPER_PROVE ``i - i2 + i2 = i:int``]);
@@ -248,6 +254,7 @@ val pat_size_lemma = prove(
 
 val pat_vars_def = tDefine "pat_vars" `
   (pat_vars (Pvar v) = [v]) /\
+  (pat_vars (Pref p) = pat_vars p) /\
   (pat_vars (Plit _) = []) /\
   (pat_vars (Pcon c xs) = FLAT (MAP pat_vars xs))`
  (WF_REL_TAC `measure (pat_size)` THEN REPEAT STRIP_TAC
@@ -301,44 +308,52 @@ val int_cmp_sem_def = Define `
 
 val get_fact_thm_T = prove(
   ``!x env.
-      evaluate' env x (Rval (Litv (Bool T))) ==>
+      evaluate' s env x (Rval (s1,Litv (Bool T))) ==>
       int_cmp_sem env T ((get_fact x))``,
   HO_MATCH_MP_TAC (fetch "-" "get_fact_ind")
   \\ FULL_SIMP_TAC std_ss [get_fact_def,int_negate_def,int_cmp_sem_def]
   \\ ONCE_REWRITE_TAC [evaluate'_cases] \\ FULL_SIMP_TAC (srw_ss()) []
   \\ SIMP_TAC (srw_ss()) [do_app_def]
   \\ REPEAT STRIP_TAC
-  \\ REPEAT (BasicProvers.FULL_CASE_TAC)
-  \\ FULL_SIMP_TAC (srw_ss()) [do_app_def] \\ TRY (Cases_on `l'`)
-  \\ FULL_SIMP_TAC (srw_ss()) [do_app_def] \\ TRY (Cases_on `l`)
-  \\ FULL_SIMP_TAC (srw_ss()) [do_app_def,evaluate_Lit]
+  \\ TRY (Cases_on `v1` \\ FULL_SIMP_TAC (srw_ss()) [])
+  \\ TRY (Cases_on `l` \\ FULL_SIMP_TAC (srw_ss()) [])
+  \\ TRY (Cases_on `v2` \\ FULL_SIMP_TAC (srw_ss()) [])
+  \\ TRY (Cases_on `l` \\ FULL_SIMP_TAC (srw_ss()) [])
   \\ Q.PAT_ASSUM `Lit xxx = e` (fn th => FULL_SIMP_TAC std_ss [GSYM th])
   \\ FULL_SIMP_TAC (srw_ss()) [opb_lookup_def,evaluate_Lit]
   \\ REPEAT (POP_ASSUM MP_TAC)
   \\ ONCE_REWRITE_TAC [evaluate'_cases] \\ FULL_SIMP_TAC (srw_ss()) []
   \\ REPEAT STRIP_TAC \\ FULL_SIMP_TAC std_ss []
-  \\ POP_ASSUM (K ALL_TAC) \\ POP_ASSUM (K ALL_TAC)
+  \\ REPEAT (Q.PAT_ASSUM `(iii:int) > jjj` MP_TAC)
+  \\ REPEAT (Q.PAT_ASSUM `(iii:int) >= jjj` MP_TAC)
+  \\ REPEAT (Q.PAT_ASSUM `(iii:int) < jjj` MP_TAC)
+  \\ REPEAT (Q.PAT_ASSUM `(iii:int) <= jjj` MP_TAC)
+  \\ REPEAT (POP_ASSUM (K ALL_TAC))
   \\ intLib.COOPER_TAC);
 
 val get_fact_thm_F = prove(
   ``!x env.
-      evaluate' env x (Rval (Litv (Bool F))) ==>
+      evaluate' s env x (Rval (s1,Litv (Bool F))) ==>
       int_cmp_sem env T (int_negate (get_fact x))``,
   HO_MATCH_MP_TAC (fetch "-" "get_fact_ind")
   \\ FULL_SIMP_TAC std_ss [get_fact_def,int_negate_def,int_cmp_sem_def]
   \\ ONCE_REWRITE_TAC [evaluate'_cases] \\ FULL_SIMP_TAC (srw_ss()) []
   \\ SIMP_TAC (srw_ss()) [do_app_def]
   \\ REPEAT STRIP_TAC
-  \\ REPEAT (BasicProvers.FULL_CASE_TAC)
-  \\ FULL_SIMP_TAC (srw_ss()) [do_app_def] \\ TRY (Cases_on `l'`)
-  \\ FULL_SIMP_TAC (srw_ss()) [do_app_def] \\ TRY (Cases_on `l`)
-  \\ FULL_SIMP_TAC (srw_ss()) [do_app_def,evaluate_Lit]
+  \\ TRY (Cases_on `v1` \\ FULL_SIMP_TAC (srw_ss()) [])
+  \\ TRY (Cases_on `l` \\ FULL_SIMP_TAC (srw_ss()) [])
+  \\ TRY (Cases_on `v2` \\ FULL_SIMP_TAC (srw_ss()) [])
+  \\ TRY (Cases_on `l` \\ FULL_SIMP_TAC (srw_ss()) [])
   \\ Q.PAT_ASSUM `Lit xxx = e` (fn th => FULL_SIMP_TAC std_ss [GSYM th])
   \\ FULL_SIMP_TAC (srw_ss()) [opb_lookup_def,evaluate_Lit]
   \\ REPEAT (POP_ASSUM MP_TAC)
   \\ ONCE_REWRITE_TAC [evaluate'_cases] \\ FULL_SIMP_TAC (srw_ss()) []
-  \\ REPEAT STRIP_TAC \\ FULL_SIMP_TAC std_ss []
-  \\ POP_ASSUM (K ALL_TAC) \\ POP_ASSUM (K ALL_TAC)
+  \\ REPEAT STRIP_TAC \\ FULL_SIMP_TAC std_ss [INT_NOT_LT,INT_NOT_LE,int_ge,int_gt]
+  \\ REPEAT (Q.PAT_ASSUM `(iii:int) > jjj` MP_TAC)
+  \\ REPEAT (Q.PAT_ASSUM `(iii:int) >= jjj` MP_TAC)
+  \\ REPEAT (Q.PAT_ASSUM `(iii:int) < jjj` MP_TAC)
+  \\ REPEAT (Q.PAT_ASSUM `(iii:int) <= jjj` MP_TAC)
+  \\ REPEAT (POP_ASSUM (K ALL_TAC))
   \\ intLib.COOPER_TAC);
 
 val decide_guard_thm = prove(
@@ -384,6 +399,7 @@ val INT_IF_OPT_def = tDefine "INT_IF_OPT" `
   (INT_IF_OPT b (Var name) = Var name) /\
   (INT_IF_OPT b (Con tag xs) = Con tag (MAP (INT_IF_OPT b) xs)) /\
   (INT_IF_OPT b (Fun name x) = Fun name x) /\
+  (INT_IF_OPT b (Uapp uop x1) = Uapp uop (INT_IF_OPT b x1)) /\
   (INT_IF_OPT b (App op x1 x2) = App op (INT_IF_OPT b x1) (INT_IF_OPT b x2)) /\
   (INT_IF_OPT b (Log l x1 x2) = Log l (INT_IF_OPT b x1) (INT_IF_OPT b x2)) /\
   (INT_IF_OPT b (If x1 x2 x3) =
@@ -443,7 +459,7 @@ val ZIP_APPEND = prove(
 
 val pmatch_lemma = prove(
    ``!p x2 env env1.
-       (pmatch' p x2 env = Match env1) ==>
+       (pmatch' s p x2 env = Match env1) ==>
        ?ys. (LENGTH ys = LENGTH (pat_vars p)) /\
             (env1 = ZIP (REVERSE (pat_vars p), ys) ++ env)``,
   STRIP_TAC \\ completeInduct_on `pat_size p` \\ REPEAT STRIP_TAC
@@ -459,28 +475,35 @@ val pmatch_lemma = prove(
   \\ FULL_SIMP_TAC (srw_ss()) [pmatch'_def,pat_vars_def,bind_def]
   \\ SRW_TAC [] [] \\ REPEAT (POP_ASSUM MP_TAC)
   \\ Q.SPEC_TAC (`l`,`l`) \\ Q.SPEC_TAC (`l'`,`l1`)
-  \\ Q.SPEC_TAC (`env`,`env`) \\ Q.SPEC_TAC (`env1`,`env1`)
-  \\ Induct_on `l` \\ Cases_on `l1` \\ FULL_SIMP_TAC std_ss [LENGTH,ADD1]
-  \\ FULL_SIMP_TAC (srw_ss()) [MAP,FLAT,LENGTH,LENGTH_NIL,ZIP,pmatch'_def]
-  \\ STRIP_TAC \\ STRIP_TAC \\ STRIP_TAC
-  \\ Cases_on `pmatch' h' h env` \\ FULL_SIMP_TAC (srw_ss()) []
-  \\ REPEAT STRIP_TAC
-  \\ FULL_SIMP_TAC std_ss [AND_IMP_INTRO]
-  \\ Q.PAT_ASSUM `!env1 env l1. bbb ==> bbbb` (MP_TAC o Q.SPECL [`env1`,`l'`,`t`])
-  \\ FULL_SIMP_TAC std_ss []
-  THEN (MATCH_MP_TAC IMP_IMP \\ STRIP_TAC THEN1
-     (REPEAT STRIP_TAC \\ FULL_SIMP_TAC std_ss [pat_size_def]
-      \\ Q.PAT_ASSUM `!x.bbb` MATCH_MP_TAC
-      \\ Q.EXISTS_TAC `x2'` \\ FULL_SIMP_TAC std_ss [] \\ DECIDE_TAC)
+  \\ Q.SPEC_TAC (`env`,`env`) \\ Q.SPEC_TAC (`env1`,`env1`) THEN1
+   (Induct_on `l` \\ Cases_on `l1` \\ FULL_SIMP_TAC std_ss [LENGTH,ADD1]
+    \\ FULL_SIMP_TAC (srw_ss()) [MAP,FLAT,LENGTH,LENGTH_NIL,ZIP,pmatch'_def]
+    \\ STRIP_TAC \\ STRIP_TAC \\ STRIP_TAC
+    \\ Cases_on `pmatch' s h' h env` \\ FULL_SIMP_TAC (srw_ss()) []
     \\ REPEAT STRIP_TAC
-    \\ Q.PAT_ASSUM `!x.bbb` (MP_TAC o Q.SPECL [`h'`,`h`,`env`])
+    \\ FULL_SIMP_TAC std_ss [AND_IMP_INTRO]
+    \\ Q.PAT_ASSUM `!env1 env l1. bbb ==> bbbb` (MP_TAC o Q.SPECL [`env1`,`l'`,`t`])
+    \\ FULL_SIMP_TAC std_ss []
+    THEN (MATCH_MP_TAC IMP_IMP \\ STRIP_TAC THEN1
+       (REPEAT STRIP_TAC \\ FULL_SIMP_TAC std_ss [pat_size_def]
+        \\ Q.PAT_ASSUM `!x.bbb` MATCH_MP_TAC
+        \\ Q.EXISTS_TAC `x2'` \\ FULL_SIMP_TAC std_ss [] \\ DECIDE_TAC)
+      \\ REPEAT STRIP_TAC
+      \\ Q.PAT_ASSUM `!x.bbb` (MP_TAC o Q.SPECL [`h'`,`h`,`env`])
+      \\ FULL_SIMP_TAC (srw_ss()) []
+      \\ MATCH_MP_TAC IMP_IMP \\ STRIP_TAC THEN1
+       (REPEAT STRIP_TAC \\ FULL_SIMP_TAC std_ss [pat_size_def] \\ DECIDE_TAC)
+      \\ REPEAT STRIP_TAC \\ FULL_SIMP_TAC std_ss []
+      \\ Q.EXISTS_TAC `ys ++ ys'`
+      \\ FULL_SIMP_TAC std_ss [LENGTH_APPEND,APPEND_ASSOC,AC ADD_ASSOC ADD_COMM]
+      \\ FULL_SIMP_TAC std_ss [ZIP_APPEND,LENGTH_REVERSE]))
+  THEN1
+   (Cases_on `store_lookup n s` \\ FULL_SIMP_TAC (srw_ss()) []
+    \\ REPEAT STRIP_TAC
+    \\ Q.PAT_ASSUM `!pp. bbb` (MP_TAC o Q.SPECL [`p'`,`x`,`env`])
     \\ FULL_SIMP_TAC (srw_ss()) []
-    \\ MATCH_MP_TAC IMP_IMP \\ STRIP_TAC THEN1
-     (REPEAT STRIP_TAC \\ FULL_SIMP_TAC std_ss [pat_size_def] \\ DECIDE_TAC)
-    \\ REPEAT STRIP_TAC \\ FULL_SIMP_TAC std_ss []
-    \\ Q.EXISTS_TAC `ys ++ ys'`
-    \\ FULL_SIMP_TAC std_ss [LENGTH_APPEND,APPEND_ASSOC,AC ADD_ASSOC ADD_COMM]
-    \\ FULL_SIMP_TAC std_ss [ZIP_APPEND,LENGTH_REVERSE]));
+    \\ MATCH_MP_TAC IMP_IMP \\ FULL_SIMP_TAC std_ss [pat_vars_def,pat_size_def]
+    \\ DECIDE_TAC)) |> GEN_ALL;
 
 val int_read_exp_IMP = prove(
   ``!x2. (int_read_exp x2 = SOME (s,r)) ==>
@@ -493,7 +516,7 @@ val int_read_exp_IMP = prove(
   \\ intLib.COOPER_TAC);
 
 val int_cmp_let_thm = prove(
-  ``EVERY (int_cmp_sem x1 T) b /\ evaluate' x1 x2 (Rval v) ==>
+  ``EVERY (int_cmp_sem x1 T) b /\ evaluate' s0 x1 x2 (Rval (s1,v)) ==>
     EVERY (int_cmp_sem (bind n v x1) T) (int_cmp_let n x2 b)``,
   SIMP_TAC std_ss [int_cmp_let_def]
   \\ Cases_on `int_read_exp x2` \\ FULL_SIMP_TAC (srw_ss()) []
@@ -503,36 +526,66 @@ val int_cmp_let_thm = prove(
   \\ REPEAT STRIP_TAC \\ Cases_on `q = s` \\ FULL_SIMP_TAC std_ss [EVERY_DEF]
   \\ FULL_SIMP_TAC std_ss [int_cmp_sem_def,bind_def,lookup_def]
   THEN (IMP_RES_TAC int_read_exp_IMP \\ FULL_SIMP_TAC std_ss []
-    \\ Q.PAT_ASSUM `evaluate' xx yy zz` MP_TAC
+    \\ Q.PAT_ASSUM `evaluate' s0 xx yy zz` MP_TAC
     \\ ASM_SIMP_TAC (srw_ss()) [Once evaluate'_cases]
     THEN1 (ONCE_REWRITE_TAC [EQ_SYM_EQ] \\ FULL_SIMP_TAC (srw_ss()) [])
     \\ REPEAT STRIP_TAC \\ IMP_RES_TAC do_app_IMP
     \\ FULL_SIMP_TAC (srw_ss()) [do_app_def,evaluate_Lit]
-    \\ Q.PAT_ASSUM `evaluate' xx yy zz` MP_TAC
+    \\ Q.PAT_ASSUM `evaluate' s0 xx yy zz` MP_TAC
     \\ Q.PAT_ASSUM `Lit xx = yy` (ASSUME_TAC o GSYM)
     \\ ASM_SIMP_TAC (srw_ss()) []
-    \\ Q.PAT_ASSUM `evaluate' xx yy zz` MP_TAC
+    \\ Q.PAT_ASSUM `evaluate' s0 xx yy zz` MP_TAC
     \\ ASM_SIMP_TAC (srw_ss()) [Once evaluate'_cases]
     \\ FULL_SIMP_TAC (srw_ss()) [opn_lookup_def,evaluate_Lit]
+    \\ ASM_SIMP_TAC (srw_ss()) [Once evaluate'_cases]
     \\ REPEAT STRIP_TAC \\ FULL_SIMP_TAC std_ss []
     \\ Q.PAT_ASSUM `-r = i2` (ASSUME_TAC o GSYM)
     \\ FULL_SIMP_TAC (srw_ss()) [evaluate_Lit]));
 
+val decide_guard_IntUnkown = prove(
+  ``!xs. decide_guard IntUnkown xs = NONE``,
+  Induct \\ FULL_SIMP_TAC std_ss [decide_guard_def]);
+
+val store_same_LEMMA = prove(
+  ``(decide_guard (get_fact x2) b = SOME x) /\
+    evaluate' s x1 x2 (Rval (s',Litv (Bool bb))) ==> (s = s')``,
+  Cases_on `x2` \\ FULL_SIMP_TAC (srw_ss()) [get_fact_def,decide_guard_IntUnkown]
+  \\ Cases_on `o'` \\ FULL_SIMP_TAC (srw_ss()) [get_fact_def,decide_guard_IntUnkown]
+  \\ Cases_on `o''` \\ FULL_SIMP_TAC (srw_ss()) [get_fact_def,decide_guard_IntUnkown]
+  \\ Cases_on `e` \\ FULL_SIMP_TAC (srw_ss()) [get_fact_def,decide_guard_IntUnkown]
+  \\ Cases_on `e0` \\ FULL_SIMP_TAC (srw_ss()) [get_fact_def,decide_guard_IntUnkown]
+  \\ TRY (Cases_on `l` \\ FULL_SIMP_TAC (srw_ss()) [get_fact_def,decide_guard_IntUnkown])
+  \\ TRY (Cases_on `l'` \\ FULL_SIMP_TAC (srw_ss()) [get_fact_def,decide_guard_IntUnkown])
+  \\ TRY (Cases_on `l` \\ FULL_SIMP_TAC (srw_ss()) [get_fact_def,decide_guard_IntUnkown])
+  \\ FULL_SIMP_TAC (srw_ss()) [do_app_def, Once evaluate'_cases]
+  \\ FULL_SIMP_TAC (srw_ss()) [do_app_def, Once evaluate'_cases]
+  \\ FULL_SIMP_TAC (srw_ss()) [do_app_def, Once evaluate'_cases]
+  \\ REPEAT STRIP_TAC
+  \\ TRY (Cases_on `v1` \\ FULL_SIMP_TAC (srw_ss()) [])
+  \\ TRY (Cases_on `v2` \\ FULL_SIMP_TAC (srw_ss()) [])
+  \\ TRY (Cases_on `l` \\ FULL_SIMP_TAC (srw_ss()) [])
+  \\ FULL_SIMP_TAC (srw_ss()) []
+  \\ REPEAT (Q.PAT_ASSUM `Lit vv = xx` (ASSUME_TAC o GSYM))
+  \\ FULL_SIMP_TAC std_ss [evaluate_Lit]);
+
 val INT_IF_OPT_LEMMA = prove(
-  ``(!x1 x2 x3. evaluate' x1 x2 x3 ==>
+  ``(!s x1 x2 x3. evaluate' s x1 x2 x3 ==>
        !b. EVERY (int_cmp_sem x1 T) b /\ isRval x3 ==>
-           evaluate' x1 (INT_IF_OPT b x2) x3) /\
-    (!x1 x2 x3. evaluate_list' x1 x2 x3 ==>
+           evaluate' s x1 (INT_IF_OPT b x2) x3) /\
+    (!s x1 x2 x3. evaluate_list' s x1 x2 x3 ==>
        !b. EVERY (int_cmp_sem x1 T) b /\ isRval x3 ==>
-           evaluate_list' x1 (MAP (INT_IF_OPT b) x2) x3) /\
-    (!x1 x2 x3 x4. evaluate_match' x1 x2 x3 x4 ==>
+           evaluate_list' s x1 (MAP (INT_IF_OPT b) x2) x3) /\
+    (!s x1 x2 x3 x4. evaluate_match' s x1 x2 x3 x4 ==>
        !b. EVERY (int_cmp_sem x1 T) b /\ isRval x4 ==>
-           evaluate_match' x1 x2 (MAT_INT_IF_OPT b x3) x4)``,
+           evaluate_match' s x1 x2 (MAT_INT_IF_OPT b x3) x4)``,
   ONCE_REWRITE_TAC [two_assums]
   \\ HO_MATCH_MP_TAC evaluate'_ind \\ REPEAT STRIP_TAC
   \\ FULL_SIMP_TAC std_ss [INT_IF_OPT_def,isRval_def]
   \\ CONV_TAC (DEPTH_CONV ETA_CONV)
   \\ TRY (RES_TAC \\ ASM_SIMP_TAC (srw_ss()) [Once evaluate'_cases] \\ NO_TAC)
+  THEN1 (RES_TAC \\ ASM_SIMP_TAC (srw_ss()) [Once evaluate'_cases] \\ METIS_TAC [])
+  THEN1 (RES_TAC \\ ASM_SIMP_TAC (srw_ss()) [Once evaluate'_cases] \\ METIS_TAC [])
+  THEN1 (RES_TAC \\ ASM_SIMP_TAC (srw_ss()) [Once evaluate'_cases] \\ METIS_TAC [])
   THEN1 (RES_TAC \\ ASM_SIMP_TAC (srw_ss()) [Once evaluate'_cases] \\ METIS_TAC [])
   THEN1 (RES_TAC \\ ASM_SIMP_TAC (srw_ss()) [Once evaluate'_cases] \\ METIS_TAC [])
   THEN1 (RES_TAC \\ ASM_SIMP_TAC (srw_ss()) [Once evaluate'_cases] \\ METIS_TAC [])
@@ -543,13 +596,13 @@ val INT_IF_OPT_LEMMA = prove(
     \\ Cases_on `op` \\ FULL_SIMP_TAC (srw_ss()) []
     \\ Cases_on `v` \\ FULL_SIMP_TAC (srw_ss()) []
     \\ Cases_on `l` \\ FULL_SIMP_TAC (srw_ss()) []
-    \\ Cases_on `b'` \\ FULL_SIMP_TAC (srw_ss()) [])
+    \\ Cases_on `b'` \\ FULL_SIMP_TAC (srw_ss()) [] \\ METIS_TAC [])
   THEN1 (ASM_SIMP_TAC (srw_ss()) [Once evaluate'_cases]
     \\ DISJ1_TAC \\ Q.EXISTS_TAC `v`
-    \\ FULL_SIMP_TAC std_ss [do_log_def])
+    \\ FULL_SIMP_TAC std_ss [do_log_def] \\ METIS_TAC [])
   THEN1 (ASM_SIMP_TAC (srw_ss()) [Once evaluate'_cases]
     \\ DISJ2_TAC \\ DISJ1_TAC \\ Q.EXISTS_TAC `v`
-    \\ FULL_SIMP_TAC std_ss [do_log_def])
+    \\ FULL_SIMP_TAC std_ss [do_log_def] \\ METIS_TAC [])
   THEN1
    (Cases_on `decide_guard (get_fact x2) b`
     \\ FULL_SIMP_TAC (srw_ss()) [] THEN1
@@ -558,15 +611,20 @@ val INT_IF_OPT_LEMMA = prove(
       \\ FULL_SIMP_TAC (srw_ss()) []
       \\ RES_TAC \\ ASM_SIMP_TAC (srw_ss()) [Once evaluate'_cases]
       \\ DISJ1_TAC \\ Q.EXISTS_TAC `v` \\ ASM_SIMP_TAC (srw_ss()) [do_if_def]
+      \\ Q.EXISTS_TAC `s'` \\ FULL_SIMP_TAC std_ss []
       THEN1 (Q.PAT_ASSUM `!b.bbb` MATCH_MP_TAC
         \\ FULL_SIMP_TAC std_ss [add_neg_fact_def,EVERY_DEF]
-        \\ MATCH_MP_TAC get_fact_thm_F \\ FULL_SIMP_TAC std_ss [])
+        \\ MATCH_MP_TAC (get_fact_thm_F |> GEN_ALL)
+        \\ FULL_SIMP_TAC std_ss [] \\ METIS_TAC [])
       THEN1 (Q.PAT_ASSUM `!b.bbb` MATCH_MP_TAC
         \\ FULL_SIMP_TAC std_ss [add_pos_fact_def,EVERY_DEF]
-        \\ MATCH_MP_TAC get_fact_thm_T \\ FULL_SIMP_TAC std_ss []))
+        \\ MATCH_MP_TAC (get_fact_thm_T |> GEN_ALL)
+        \\ FULL_SIMP_TAC std_ss [] \\ METIS_TAC []))
     \\ IMP_RES_TAC decide_guard_thm
     \\ FULL_SIMP_TAC std_ss [do_if_def]
     \\ Cases_on `v = Litv (Bool T)` \\ FULL_SIMP_TAC std_ss []
+    \\ `s' = s` by METIS_TAC [store_same_LEMMA]
+    \\ FULL_SIMP_TAC std_ss []
     THEN1 (Cases_on `x` \\ FULL_SIMP_TAC (srw_ss()) []
       \\ IMP_RES_TAC get_fact_thm_T
       \\ IMP_RES_TAC decide_guard_IMP
@@ -581,15 +639,19 @@ val INT_IF_OPT_LEMMA = prove(
   THEN1 (RES_TAC \\ ASM_SIMP_TAC (srw_ss()) [Once evaluate'_cases] \\ METIS_TAC [])
   THEN1 (RES_TAC \\ ASM_SIMP_TAC (srw_ss()) [Once evaluate'_cases] \\ METIS_TAC [])
   THEN1 (RES_TAC \\ ASM_SIMP_TAC (srw_ss()) [Once evaluate'_cases]
-    \\ DISJ1_TAC \\ Q.EXISTS_TAC `v` \\ FULL_SIMP_TAC std_ss []
+    \\ DISJ1_TAC \\ Q.LIST_EXISTS_TAC [`v`,`s'`] \\ FULL_SIMP_TAC std_ss []
     \\ Q.PAT_ASSUM `!b.bbb` MATCH_MP_TAC
     \\ FULL_SIMP_TAC std_ss [EVERY_APPEND]
     \\ FULL_SIMP_TAC std_ss [EVERY_FILTER,int_cmp_let_thm]
+    \\ IMP_RES_TAC int_cmp_let_thm
+    \\ FULL_SIMP_TAC std_ss []
     \\ FULL_SIMP_TAC std_ss [EVERY_MEM]
     \\ REPEAT STRIP_TAC \\ RES_TAC
     \\ Cases_on `x`
     \\ FULL_SIMP_TAC std_ss [int_cmp_sem_def,int_cmp_keep_def]
     \\ Q.EXISTS_TAC `j` \\ FULL_SIMP_TAC std_ss [MEM,lookup_def,bind_def])
+  THEN1 (RES_TAC \\ ASM_SIMP_TAC (srw_ss()) [Once evaluate'_cases] \\ METIS_TAC [])
+  THEN1 (RES_TAC \\ ASM_SIMP_TAC (srw_ss()) [Once evaluate'_cases] \\ METIS_TAC [])
   THEN1 (RES_TAC \\ ASM_SIMP_TAC (srw_ss()) [Once evaluate'_cases] \\ METIS_TAC [])
   THEN1 (RES_TAC \\ ASM_SIMP_TAC (srw_ss()) [Once evaluate'_cases] \\ METIS_TAC [])
   THEN1 (FULL_SIMP_TAC std_ss [MAT_INT_IF_OPT_def,MAP]
@@ -603,16 +665,17 @@ val INT_IF_OPT_LEMMA = prove(
       \\ Cases_on `x`
       \\ FULL_SIMP_TAC std_ss [int_cmp_sem_def,int_cmp_keep_def]
       \\ Q.EXISTS_TAC `j` \\ FULL_SIMP_TAC std_ss []
-      \\ `~MEM s (REVERSE (pat_vars p))` by FULL_SIMP_TAC std_ss [MEM_REVERSE]
+      \\ `~MEM s' (REVERSE (pat_vars p))` by FULL_SIMP_TAC std_ss [MEM_REVERSE]
       \\ FULL_SIMP_TAC std_ss [lookup_ZIP_APPEND,LENGTH_REVERSE])
   THEN1
      (FULL_SIMP_TAC std_ss [MAT_INT_IF_OPT_def,MAP]
-      \\ ASM_SIMP_TAC (srw_ss()) [Once evaluate'_cases]));
+      \\ ASM_SIMP_TAC (srw_ss()) [Once evaluate'_cases] \\ METIS_TAC []));
 
 val INT_IF_OPT_THM =
-  INT_IF_OPT_LEMMA |> CONJUNCT1 |> Q.SPECL [`env`,`exp`,`Rval res`]
+  INT_IF_OPT_LEMMA |> CONJUNCT1 |> Q.SPECL [`s`,`env`,`exp`,`Rval res`]
     |> SIMP_RULE std_ss [isRval_def,PULL_FORALL] |> Q.SPEC `[]`
-    |> REWRITE_RULE [EVERY_DEF] |> Q.GEN `res` |> Q.GEN `exp` |> Q.GEN `env`
+    |> REWRITE_RULE [EVERY_DEF]
+    |> Q.GEN `res` |> Q.GEN `exp` |> Q.GEN `env` |> Q.GEN `s`
 
 
 (* top-level optimiser *)
